veric/null_extension.v
@@ -6,217 +6,297 @@ Require Import msl.base
 Set Implicit Arguments.
 
 Section NullExtension.
- Variables 
-  (F V cT D Z: Type) 
-  (ge: Genv.t F V)
-  (csem: CoreSemantics (Genv.t F V) cT mem D)
-  (csig: ext_sig mem Z)
+ Variables
+  (fT vT cT dT Z: Type) (** external states *)
+  (csemT: CoreSemantics (Genv.t fT vT) cT mem dT) 
+  (csig: ext_sig mem Z) (** client signature *)
+  (genv_mapT: forall i:nat, Genv.t fT vT)
   (init_world: Z)
   (at_external_handled: forall c ef args sig,
-    at_external csem c = Some (ef, sig, args) -> IN ef csig = true).
+    at_external csemT c = Some (ef, sig, args) -> IN ef csig = true).
 
-Definition cores := fun _:nat => Some csem.
+ Definition cores := fun _:nat => csemT.
 
-Local Open Scope nat_scope.
+ Local Open Scope nat_scope.
 
-Definition proj_core (i: nat) (c: cT) := if eq_nat_dec i 1 then Some c else None.
-Definition active := fun _: cT => 1.
-Definition runnable := fun (s: cT) => 
-  match at_external csem s, safely_halted csem s with 
-  | None, None => true
-  | _, _ => false
-  end.
-Definition proj_zint := fun _: cT => tt.
-Definition proj_zext := fun z: Z => z.
-Definition zmult := fun (_: unit) (z: Z) => z.
-Definition handled: list AST.external_function := nil.
+ Definition xT := cT.
+ Definition proj_core (i: nat) (s: xT) := if eq_nat_dec i 0 then Some s else None.
+ Definition active := fun _:xT => 0.
+ Definition runnable := fun (s: xT) => 
+   match at_external csemT s, safely_halted csemT s with 
+     | None, None => true
+     | _, _ => false
+   end.
+ Definition proj_zint := fun _:xT => tt.
+ Definition proj_zext := fun z: Z => z.
+ Definition zmult := fun (_:unit) (z: Z) => z.
+ Definition handled: list AST.external_function := nil.
 
-Local Hint Unfold cores proj_core active runnable proj_zint : null_unfold.
+ Local Hint Unfold cores proj_core active runnable proj_zint : null_unfold.
 
-Obligation Tactic := 
-  autounfold with null_unfold;
-  intros; try solve [eexists; eauto|congruence].
+ Obligation Tactic := 
+   autounfold with null_unfold;
+   intros; try solve [eexists; eauto|congruence].
 
-Program Definition null_extension := Extension.Make 
-  _
-  csem cores csig csig handled
+ Definition fT' := fun i:nat => fT.
+ Definition vT' := fun i:nat => vT.
+ 
+ Program Definition null_extension := Extension.Make 
+  (fun i:nat => Genv.t (fT' i) (vT' i))
+  csemT cores csig csig handled
   proj_core _  
-  active _ _
+  active _ 
   runnable _ _ _ _  
   proj_zint proj_zext zmult _ _ _.
-Next Obligation.
-revert H0; case_eq (eq_nat_dec i 1).
-intros -> _; exists s; auto.
-congruence.
-Qed.
-Next Obligation.
-if_tac; exists s; auto.
-elimtype False; apply H; auto.
-Qed.
-Next Obligation. 
-if_tac in H1; try congruence; inv H1; inv H0.
-destruct (at_external CS c); try solve[congruence].
-destruct p as [[? ?] ?]. 
-right; eexists; eexists; eexists; eauto.
-destruct (safely_halted CS c); try solve[congruence].
-left; eexists; eauto.
-Qed.
-Next Obligation. inversion H; subst; eapply at_external_handled; eauto. Qed.
-Next Obligation. inversion H; subst; if_tac in H0; try congruence. Qed.
-Next Obligation. unfold linkable; intros; inv H0; inv H1; exists x'; auto. Qed.
+ Next Obligation.
+   revert H0; case_eq (eq_nat_dec i 0).
+   intros -> _; exists s; auto.
+   congruence.
+ Qed.
+ Next Obligation.
+   if_tac; exists s; auto.
+   elimtype False; apply H; auto.
+ Qed.
+ Next Obligation. 
+   if_tac in H0; try congruence; inv H0; inv H.
+   unfold fT', vT' in *.
+   destruct (at_external csemT c); try solve[congruence].
+   destruct p as [[? ?] ?]. 
+   right; eexists; eexists; eexists; eauto.
+   destruct (safely_halted csemT c); try solve[congruence].
+   solve[left; eexists; eauto].
+ Qed.
+ Next Obligation. inversion H; subst; eapply at_external_handled; eauto. Qed.
+ Next Obligation. 
+  inversion H; subst; if_tac in H; try congruence. 
+  unfold fT', vT' in *.
+  inversion H3; subst.
+  solve[rewrite H0 in H1; congruence].
+ Qed.
+ Next Obligation. unfold linkable; intros; inv H0; inv H1; exists x'; auto. Qed.
 
 End NullExtension.
 
 Section NullExtensionSafe.
- Variables 
-  (F V cT D Z: Type) 
-  (ge: Genv.t F V)
-  (csem: CoreSemantics (Genv.t F V) cT mem D)
-  (csig: ext_sig mem Z)
+ Variables
+  (fT vT cT dT Z: Type) (** external states *)
+  (csemT: CoreSemantics (Genv.t fT vT) cT mem dT) 
+  (csig: ext_sig mem Z) (** client signature *)
+  (genv_mapT: forall i:nat, Genv.t fT vT)
   (init_world: Z)
   (at_external_handled: forall c ef args sig,
-    at_external csem c = Some (ef, sig, args) -> IN ef csig = true).
+    at_external csemT c = Some (ef, sig, args) -> IN ef csig = true)
+  (ge: Genv.t fT vT).
 
-Import ExtensionSafety.
+ Import ExtensionSafety.
 
-Local Hint Unfold cores proj_core active runnable proj_zint : null_unfold.
+ Local Hint Unfold cores proj_core active runnable proj_zint : null_unfold.
 
-Obligation Tactic := 
-  autounfold with null_unfold;
-  intros; try solve [eexists; eauto|congruence].
+ Obligation Tactic := 
+   autounfold with null_unfold;
+   intros; try solve [eexists; eauto|congruence].
 
-Lemma null_extension_safe (csem_fun: corestep_fun csem): 
- safe_extension ge (fun _:nat => ge) (null_extension csem csig at_external_handled).
-Proof.
-destruct (ExtensionSafety (null_extension csem csig at_external_handled) 
+ Lemma null_extension_safe (csem_fun: corestep_fun csemT): 
+  safe_extension ge (fun _:nat => ge) (null_extension csemT csig at_external_handled).
+ Proof.
+ destruct (ExtensionSafety (null_extension csemT csig at_external_handled) 
   ge (fun _:nat => ge)) as [PF].
-apply PF.
-constructor; autounfold with null_unfold in *.
+ apply PF.
+ constructor; autounfold with null_unfold in *.
 
-(*1*) intros until m'; intros H1 [H3 H4] H5 H6. 
-inversion H3 as [H7]; rewrite <-H7 in *; clear H7 H3.
-unfold Extension.proj_core in H4; simpl in H4.
-generalize H4 as H4'; intro.
-unfold proj_core in H4; if_tac in H4; try solve[congruence].
-inversion H4 as [H7]; rewrite H7 in *; clear H7 H4.
-rewrite H in *; clear H.
-unfold Extension.proj_core; simpl; unfold proj_core.
-simpl in H5.
-f_equal; generalize (csem_fun _ _ _ _ _ _ _ H5 H6); inversion 1; auto.
-simpl in H1|-*.
-unfold proj_zint, all_safe in *.
-intros until c0; intros H0 H8.
-inversion H0 as [H7]; rewrite H7 in *; clear H0.
-unfold Extension.proj_core in H8; simpl in H8; unfold proj_core in H8.
-if_tac in H8; try solve[congruence].
-rewrite <-H0 in *; clear H; inversion H8 as [H].
-rewrite H in *; clear H8 H.
-solve[eapply safe_corestep_forward; eauto].
+ (*1*) intros until m'; intros H1 H4 H5 H6. 
+ assert (H3:True) by auto.
+ unfold Extension.proj_core in H4; simpl in H4.
+ generalize H4 as H4'; intro.
+ unfold proj_core in H4; if_tac in H4; try solve[congruence].
+ inversion H4 as [H7]; rewrite H7 in *; clear H7 H4.
+ rewrite H in *; clear H.
+ unfold Extension.proj_core; simpl; unfold proj_core.
+ simpl in H5.
+ f_equal; generalize (csem_fun _ _ _ _ _ _ _ H5 H6); inversion 1; auto.
+ simpl in H1|-*.
+ unfold proj_zint, all_safe in *.
+ intros until c0; intros H0.
+ assert (H8:True) by auto.
+ inversion H0 as [H7]. simpl in H0. rewrite H7 in *; clear H0.
+ unfold proj_core in H7.
+ if_tac in H7; try solve[congruence].
+ rewrite <-H0 in *; clear H; inversion H7 as [H].
+ rewrite H in *; clear H7 H.
+ solve[eapply safe_corestep_forward; eauto].
 
-(*2*) intros until CS; intros H1 H3 [H4 H5].
-spec H1 (active s) CS c H4 H5.
-simpl in H5.
-simpl in H3; unfold runnable in H3; simpl in H3.
-case_eq (at_external csem s).
-intros [[ef sig] args] H6.
-rewrite H6 in H3.
-simpl in H5; unfold proj_core in H5; simpl in H5; inversion H5; subst.
-congruence.
-intros H6.
-rewrite H6 in H3.
-unfold proj_core in H5.
-if_tac in H5; try congruence.
-inv H5.
-case_eq (safely_halted csem c); try congruence.
-intros rv Hsafe.
-rewrite Hsafe in H3.
-congruence.
-simpl in H1.
-inversion H4.
-rewrite <-H2 in *.
-rewrite H6 in H1.
-intros Hsafe; rewrite Hsafe in H1.
-destruct H1 as [c' [m' [H1 H7]]].
-solve[exists c'; exists c'; exists m'; split; auto].
+ (*2*) intros until c; intros H1 H3 H5.
+ assert (H4:True) by auto.
+ spec H1 (active s) c H5.
+ simpl in H5.
+ simpl in H3; unfold runnable in H3; simpl in H3.
+ case_eq (at_external csemT s).
+ intros [[ef sig] args] H6.
+ rewrite H6 in H3.
+ simpl in H5; unfold proj_core in H5; simpl in H5; inversion H5; subst.
+ congruence.
+ intros H6.
+ rewrite H6 in H3.
+ unfold proj_core in H5.
+ if_tac in H5; try congruence.
+ inv H5.
+ case_eq (safely_halted csemT c); try congruence.
+ intros rv Hsafe.
+ rewrite Hsafe in H3.
+ congruence.
+ unfold fT', vT' in *.
+ simpl in H1.
+ rewrite H6 in H1.
+ intros Hsafe; rewrite Hsafe in H1.
+ destruct H1 as [c' [m' [H1 H7]]].
+ solve[exists c'; exists c'; exists m'; split; auto].
 
-(*3*) intros until x; intros [H1 H2] H3 H4 H5 H6 H7 H8.
-apply ListSet.set_mem_correct1 in H4.
-unfold handled, ListSet.set_In in H4.
-solve[inversion H4].
+ (*3*) intros until x; intros H2 H3 H4 H5 H6 H7 H8.
+ assert (H1:True) by auto.
+ apply ListSet.set_mem_correct1 in H4.
+ unfold handled, ListSet.set_In in H4.
+ solve[inversion H4].
 
-(*4*) intros until m; intros H1 H2 H3.
-simpl in H2; unfold runnable in H2.
-inversion H3; subst.
-unfold compose in H0;  simpl in H0.
-rewrite H0 in H2.
-case_eq (safely_halted csem s); intros; try solve[congruence].
-rewrite H in H2.
-right; exists v; auto.
-solve[rewrite H in H2; congruence].
+ (*4*) intros until m; intros H1 H2 H3.
+ simpl in H2; unfold runnable in H2.
+ inversion H3; subst.
+ unfold compose in H0;  simpl in H0.
+ rewrite H0 in H2.
+ case_eq (safely_halted csemT s); intros; try solve[congruence].
+ rewrite H in H2.
+ right; exists v; auto.
+ solve[rewrite H in H2; congruence].
 
-(*5*) intros until rv; intros [H1 H2] H3 H4.
-split; auto.
-simpl.
-apply corestep_not_halted in H4.
-simpl in H2; inversion H2; subst.
-inversion H1; rewrite H5 in *.
-unfold proj_core in H0.
-solve[if_tac in H0; try solve[congruence]].
+ (*5*) intros until rv; intros H2 H3 H4.
+ unfold fT', vT' in *.
+ simpl.
+ apply corestep_not_halted in H4.
+ simpl in H2; inversion H2; subst.
+ unfold proj_core in H0.
+ solve[if_tac in H0; try solve[congruence]].
 
-(*6*) intros until CS; inversion 1; subst.
-intros H4 H5; intros until j; intros H6; split.
-intros [H7 H8]. 
-split; auto.
-simpl in H8; unfold proj_core in H8; simpl in H8; inversion H8; subst.
-simpl; unfold proj_core; simpl.
-simpl in H6; unfold active in H6.
-if_tac; auto.
-exfalso; apply H3; auto.
-intros n z z' [H7 H8].
-simpl in H8; unfold proj_core in H8; simpl in H8.
-simpl in H6; unfold active in H6; simpl in H6.
-if_tac in H8; auto.
-inversion H8; subst.
-exfalso; apply H3; auto.
-solve[congruence].
+ (*6*) intros until c; inversion 1; subst.
+ intros H4 H5; intros until c0; intros H6; split.
+ intros H8.
+ assert (H7:True) by auto.
+ simpl in H8; unfold proj_core in H8; simpl in H8; inversion H8; subst.
+ simpl; unfold proj_core; simpl.
+ simpl in H6; unfold active in H6.
+ if_tac; auto.
+ exfalso; apply H6; auto.
+ intros n z z' H8.
+ assert (H7:True) by auto.
+ simpl in H8; unfold proj_core in H8; simpl in H8.
+ simpl in H6; unfold active in H6; simpl in H6.
+ if_tac in H8; auto.
+ inversion H8; subst.
+ exfalso; apply H6; auto.
+ solve[congruence].
 
-(*7*) exists csem; exists s; split; auto. 
+ (*7*) intros until args; intros H1.
+ solve[exists s; split; auto].
 
-(*8*) intros until Q.
-intros [H1 H2] H3 H4 H5 H6.
-intros H12; simpl; exists c'; split3; auto.
-simpl in H2; unfold proj_core in H2.
-if_tac in H2; try solve[congruence].
+ (*8*) intros until Q.
+ unfold fT', vT' in *.
+ intros H2 H3 H4 H5 H6.
+ assert (H1:True) by auto.
+ intros H12; simpl; exists c'; split3; auto.
+ simpl in H2; unfold proj_core in H2.
+ if_tac in H2; try solve[congruence].
 
-(*9*) intros until Q; intros [H1 H2] H3 H4 H5 H6 H7 H70 [H8 H9]; 
- intros until j; intros H10; split.
-intros [H11 H12].
-simpl in H12; unfold proj_core in H12; simpl in H12.
-if_tac in H12; auto.
-simpl in H9; unfold proj_core in H9; simpl in H9.
-simpl in H10; unfold active in H10; simpl in H10.
-exfalso; apply H; auto.
-congruence.
-intros ge'  n [H11 H12].
-simpl in H10, H12.
-unfold active in H10; unfold proj_core in H12.
-if_tac in H12.
-exfalso; auto.
-congruence.
-Qed.
+ (*9*) intros until Q; intros H2 H3 H4 H5 H6 H7 H70 [H8 H9]; 
+ intros until c0; intros H10; split.
+ intros H12.
+ assert (H11:True) by auto.
+ simpl in H12; unfold proj_core in H12; simpl in H12.
+ if_tac in H12; auto.
+ simpl in H9; unfold proj_core in H9; simpl in H9.
+ simpl in H10; unfold active in H10; simpl in H10.
+ exfalso; apply H10; auto.
+ congruence.
+ intros ge'  n H12.
+ simpl in H10, H12.
+ unfold active in H10; unfold proj_core in H12.
+ if_tac in H12.
+ exfalso; auto.
+ congruence.
+ Qed.
 
 End NullExtensionSafe.
 
+(*
+  (F V fS fT vS vT: Type) (** global environments *)
+  (cS cT: Type) (** corestates of source and target core semantics *)
+  (dS dT: Type) (** initialization data *)
+  (Z: Type) (** external states *)
+  (Zint: Type) (** portion of Z implemented by extension *)
+  (Zext: Type) (** portion of Z external to extension *)
+  (esemS: CoreSemantics (Genv.t F V) cS mem dS) (** extended source semantics *)
+  (esemT: CoreSemantics (Genv.t F V) cT mem dT) (** extended target semantics *)
+  (csemS: CoreSemantics (Genv.t fS vS) cS mem dS) 
+  (csemT: CoreSemantics (Genv.t fT vT) cT mem dT) 
+  (csig: ext_sig mem Z) (** client signature *)
+  (esig: ext_sig mem Zext) (** extension signature *)
+  (handled: list AST.external_function). (** functions handled by this extension *)
+
+ Variables 
+  (ge: Genv.t F V) (geS: Genv.t fS vS) (geT: Genv.t fT vT).
+
+ Variable (E_S: Extension.Sig (fun i => Genv.t ((fun _ => fS) i) ((fun _ => vS) i)) 
+                  (fun _ => cS) Zint esemS (fun i:nat => Some ((fun _ => csemS) i)) 
+                  csig esig handled).
+ Variable (E_T: Extension.Sig (fun i => Genv.t ((fun _ => fT) i) ((fun _ => vT) i)) 
+                  (fun _ => cT) Zint esemT (fun i:nat => Some ((fun _ => csemT) i)) 
+                  csig esig handled).
+
+ Variable entry_points: list (val*val*signature).
+
+ Import Sim_inj.
+
+ Variable max_threads: nat.
+
+ Variable core_simulations: forall i:nat, 
+   Forward_simulation_inject dS dT csemS csemT geS geT entry_points.
+*)
+(*
 Section NullExtensionCompilable.
  Variables 
-  (F_S V_S cS dS F_T V_T cT dT Z: Type) 
-  (csemS: CoreSemantics (Genv.t F_S V_S) cS mem dS)
-  (csemT: CoreSemantics (Genv.t F_T V_T) cT mem dT)
+  (F V fS vS fT vT cS cT dS dT Z: Type) 
   (csig: ext_sig mem Z)
   (init_world: Z)
+  (entry_points: list (val*val*signature))
+  (csemS: CoreSemantics (Genv.t fS vS) cS mem dS)
+  (csemT: CoreSemantics (Genv.t fT vT) cT mem dT)
   (at_external_handledS: forall c ef args sig,
     at_external csemS c = Some (ef, sig, args) -> IN ef csig = true)
   (at_external_handledT: forall c ef args sig,
     at_external csemT c = Some (ef, sig, args) -> IN ef csig = true).
 
+ Variables (ge: Genv.t F V) (geS: Genv.t fS vS) (geT: Genv.t fT vT).
+
+ Definition E_S: 
+  Extension.Sig (fun i : nat => Genv.t ((fun _ => fS) i) ((fun _ => vS) i))
+   (fun _ : nat => cS) unit csemS (fun _:nat => csemS) csig csig handled := 
+  null_extension csemS csig at_external_handledS.
+ Definition E_T: 
+  Extension.Sig (fun i : nat => Genv.t ((fun _ => fT) i) ((fun _ => vT) i))
+   (fun _ : nat => cT) unit csemT (fun _:nat => csemT) csig csig handled := 
+ null_extension csemT csig at_external_handledT.
+
+ Import Sim_inj.
+
+ Variable core_simulations: forall i:nat,
+  Forward_simulation_inject dS dT csemS csemT geS geT entry_points.
+
+ Definition genv_mapS := fun i:nat => geS.
+ Definition genv_mapT := fun i:nat => geT.
+Set Printing All.
+Check CompilableExtension.Sig.
+ Lemma null_extension_compilable:
+   @CompilableExtension.Sig F V cS cT 
+    (fun _ => fS) (fun _ => fT) (fun _ => vS) (fun _ => vT) (fun _ => cS) (fun _ => cT)
+    dS dT Z unit Z csemS csemT (fun _ => csemS) (fun _ => csemT)
+    ge genv_mapS genv_mapT E_S E_T core_simulations.
+
 End NullExtensionCompilable.
+*)
